lemmas characterizing between as Abs. bound on Abs of integral based on bounds on the Abs of derivatives
since the exists in changesTo is prop, things using it are supposed to be
in Prop. Tried to switch it to Type. However, many things broke.
One has toe change the definition of Device, or node semantics

icreate.v
@@ -1219,6 +1219,30 @@ Proof.
   rewrite inj_Q_Zero. reflexivity.
 Qed.
 
+Definition optimalTurnAngle : IR :=
+  CRasIR (θ (Cart2Polar targetPos)).
+
+Definition turnAcc : IR.
+Admitted.
+
+Lemma OmegaThetaPosAtEV1 :
+  let t0 : QTime := MotorEventsNthTime 0 (decAuto (0<4)%nat I) in
+  let t1 : QTime := MotorEventsNthTime 1 (decAuto (1<4)%nat I) in
+     |{theta icreate} t1 - optimalTurnAngle| ≤ turnAcc.
+Proof.
+  intros ? ?.
+  pose proof correctVel0to1 as Hc.
+  simpl in Hc. fold t0 in Hc.
+  unfold correctVelDuring in Hc.
+  apply proj2 in Hc. simpl θ in Hc.
+  fold t1 in Hc.
+  match type of Hc with
+  context[omegaPrec ?om]
+    => remember (omegaPrec om) as opr
+  end.
+Abort.
+  
+
 Lemma TurnCompleteTime :
   ∃ (t : QTime), 
       ((|({theta icreate} t) - CRasIR (θ (Cart2Polar targetPos))|) ≤ [0]).
